src/lowparse/LowParse.Low.ConstInt32.fst
@@ -12,29 +12,33 @@ module U32 = FStar.UInt32
 module HS = FStar.HyperStack
 module HST = FStar.HyperStack.ST
 
-(*
 let valid_constint32le
-  (v: nat { 0 <= v /\ v < 4294967276 } )
+  (v: nat { 0 <= v /\ v < 4294967296 } )
   (h: HS.mem)
   (#rrel #rel: _)
   (input: slice rrel rel)
   (pos: U32.t)
 : Lemma (valid (parse_constint32le v) h input pos 
     <==> 
-    (live_slice h input /\ 
-    U32.v input.len - U32.v pos >= 4 /\
-    U32.v (contents (parse_constint32le v) h input pos) == v))
-= valid_facts (parse_constint32le v) h input pos
-*)
+    (valid (parse_int32_le ()) h input pos /\
+    U32.v (contents (parse_int32_le ()) h input pos) == v))
+= valid_facts (parse_constint32le v) h input pos;
+  valid_facts (parse_int32_le ()) h input pos;
+  parse_constint32le_unfold v (bytes_of_slice_from h input pos)
 
-#push-options "--z3rlimit 40"
+let read_int32_le : unit -> Tot (leaf_reader (parse_int32_le ()))
+= read_bounded_integer_le_4
 
-let validate_constint32le
-  (v: U32.t)
+(*
+let validate_constint32le_slow
+  (v: U32.t { 0 <= U32.v v /\ U32.v v < 4294967296 } )
 : Tot (validator (parse_constint32le (U32.v v)))
 = fun #rrel #rel (input: slice rrel rel) (pos: U32.t) ->
   let h = HST.get() in
-    let _ = valid_equiv (parse_constint32le (U32.v v)) h input pos in
+    let _ =
+      valid_equiv (parse_constint32le (U32.v v)) h input pos;
+      valid_constint32le (U32.v v) h input pos    
+    in
   if U32.lt (input.len `U32.sub` pos) 4ul
   then
     validator_error_not_enough_data
@@ -44,5 +48,4 @@ let validate_constint32le
       pos `U32.add` 4ul
     else
       validator_error_generic
-   
-#pop-options
+*)
